Refactor multi-universe classes to use target universes

UniverseAbstractions/Axioms/Universe/Equivalences.lean
@@ -11,35 +11,38 @@ import UniverseAbstractions.Lemmas.DerivedProductFunctors
 set_option autoBoundImplicitLocal false
 --set_option pp.universes true
 
-universe u v w w'
+universe u v w w' w''
 
 
 
-class HasExternalEquivalence {U : Universe.{u}} {V : Universe.{v}} (α : U) (β : V)
-                             [HasExternalFunctor.{u, v, w} α β] [HasExternalFunctor.{v, u, w} β α] where
-(IsEquiv : (α ⟶' β) → (β ⟶' α) → Sort w')
+class HasEquivalenceCondition (U : Universe.{u}) (V : Universe.{v})
+                              [HasFunctoriality.{u, v, w} U V] [HasFunctoriality.{v, u, w} V U] where
+(IsEquiv {α : U} {β : V} : (α ⟶' β) → (β ⟶' α) → Sort w')
 
-namespace HasExternalEquivalence
+namespace HasEquivalenceCondition
 
-  def DefEquiv {U : Universe.{u}} {V : Universe.{v}} (α : U) (β : V)
-               [HasExternalFunctor.{u, v, w} α β] [HasExternalFunctor.{v, u, w} β α]
-               [h : HasExternalEquivalence.{u, v, w, w'} α β] (toFun : α ⟶' β) (invFun : β ⟶' α) :=
+  variable {U : Universe.{u}} {V : Universe.{v}}
+           [HasFunctoriality.{u, v, w} U V] [HasFunctoriality.{v, u, w} V U]
+           [h : HasEquivalenceCondition.{u, v, w, w'} U V]
+
+  def DefEquiv {U : Universe.{u}} {V : Universe.{v}}
+               [HasFunctoriality.{u, v, w} U V] [HasFunctoriality.{v, u, w} V U]
+               [h : HasEquivalenceCondition.{u, v, w, w'} U V]
+               (α : U) (β : V) (toFun : α ⟶' β) (invFun : β ⟶' α) :=
   h.IsEquiv toFun invFun
 
-  notation:20 α:21 " ⟷'[" toFun:0 "," invFun:0 "] " β:21 => HasExternalEquivalence.DefEquiv α β toFun invFun
+  notation:20 α:21 " ⟷'[" toFun:0 "," invFun:0 "] " β:21 => HasEquivalenceCondition.DefEquiv α β toFun invFun
 
-  structure Equiv {U : Universe.{u}} {V : Universe.{v}} (α : U) (β : V)
-                  [HasExternalFunctor.{u, v, w} α β] [HasExternalFunctor.{v, u, w} β α]
-                  [HasExternalEquivalence.{u, v, w, w'} α β] : Sort (max 1 u v w w') where
+  structure Equiv {U : Universe.{u}} {V : Universe.{v}}
+                  [HasFunctoriality.{u, v, w} U V] [HasFunctoriality.{v, u, w} V U]
+                  [HasEquivalenceCondition.{u, v, w, w'} U V] (α : U) (β : V) : Sort (max 1 u v w w') where
   (toFun  : α ⟶' β)
   (invFun : β ⟶' α)
   (E      : α ⟷'[toFun,invFun] β)
 
-  infix:20 " ⟷' " => HasExternalEquivalence.Equiv
+  infix:20 " ⟷' " => HasEquivalenceCondition.Equiv
 
-  variable {U : Universe.{u}} {V : Universe.{v}} {α : U} {β : V}
-           [HasExternalFunctor.{u, v, w} α β] [HasExternalFunctor.{v, u, w} β α]
-           [HasExternalEquivalence.{u, v, w, w'} α β]
+  variable {α : U} {β : V}
 
   def toDefEquiv                                      (E : α ⟷' β)               : α ⟷'[E.toFun,E.invFun] β := E.E
   def fromDefEquiv {toFun : α ⟶' β} {invFun : β ⟶' α} (E : α ⟷'[toFun,invFun] β) : α ⟷'                   β := ⟨toFun, invFun, E⟩
@@ -51,176 +54,170 @@ namespace HasExternalEquivalence
   match E with | ⟨_, _, _⟩ => rfl
   @[simp] theorem toFromDefEquiv {toFun : α ⟶' β} {invFun : β ⟶' α} (E : α ⟷'[toFun,invFun] β) : toDefEquiv (fromDefEquiv E) = E := rfl
 
-end HasExternalEquivalence
+end HasEquivalenceCondition
 
 
 
-class HasIdEquiv {U : Universe} (α : U) [HasExternalFunctor α α] [HasIdFun α] [HasExternalEquivalence α α] where
-(defIdEquiv: α ⟷'[HasIdFun.idFun α, HasIdFun.idFun α] α)
+class HasIdEquiv (U : Universe) [HasFunctoriality U U] [HasIdFun U] [HasEquivalenceCondition U U] where
+(defIdEquiv (α : U) : α ⟷'[HasIdFun.idFun' α, HasIdFun.idFun' α] α)
 
 namespace HasIdEquiv
 
-  variable {U : Universe} (α : U) [HasExternalFunctor α α] [HasIdFun α] [HasExternalEquivalence α α] [HasIdEquiv α]
+  variable {U : Universe} [HasFunctoriality U U] [HasIdFun U] [HasEquivalenceCondition U U] [HasIdEquiv U]
 
-  def idEquiv : α ⟷' α := HasExternalEquivalence.fromDefEquiv defIdEquiv
+  def idEquiv' (α : U) : α ⟷' α := HasEquivalenceCondition.fromDefEquiv (defIdEquiv α)
 
 end HasIdEquiv
 
-class HasInvEquiv {U V : Universe} (α : U) (β : V) [HasExternalFunctor α β] [HasExternalFunctor β α]
-                  [HasExternalEquivalence α β] [HasExternalEquivalence β α] where
-(defInvEquiv (E : α ⟷' β) : β ⟷'[E.invFun, E.toFun] α)
-
-class HasCompEquiv {U V W : Universe} (α : U) (β : V) (γ : W) 
-                   [HasExternalFunctor α β] [HasExternalFunctor β γ] [HasExternalFunctor α γ]
-                   [HasExternalFunctor β α] [HasExternalFunctor γ β] [HasExternalFunctor γ α]
-                   [HasCompFun α β γ] [HasCompFun γ β α]
-                   [HasExternalEquivalence α β] [HasExternalEquivalence β γ] [HasExternalEquivalence α γ] where
-(defCompEquiv (E : α ⟷' β) (F : β ⟷' γ) : α ⟷'[F.toFun ⊙' E.toFun, E.invFun ⊙' F.invFun] γ)
-
-namespace HasCompEquiv
-
-  variable {U V W : Universe} {α : U} {β : V} {γ : W}
-           [HasExternalFunctor α β] [HasExternalFunctor β γ] [HasExternalFunctor α γ]
-           [HasExternalFunctor β α] [HasExternalFunctor γ β] [HasExternalFunctor γ α]
-           [HasCompFun α β γ] [HasCompFun γ β α]
-           [HasExternalEquivalence α β] [HasExternalEquivalence β γ] [HasExternalEquivalence α γ]
-           [HasCompEquiv α β γ]
-
-  def compEquiv (E : α ⟷' β) (F : β ⟷' γ) : α ⟷' γ := HasExternalEquivalence.fromDefEquiv (defCompEquiv E F)
-
-end HasCompEquiv
+class HasInvEquiv (U V : Universe) [HasFunctoriality U V] [HasFunctoriality V U]
+                  [HasEquivalenceCondition U V] [HasEquivalenceCondition V U] where
+(defInvEquiv {α : U} {β : V} (E : α ⟷' β) : β ⟷'[E.invFun, E.toFun] α)
 
 namespace HasInvEquiv
 
-  variable {U V : Universe} {α : U} {β : V} [HasExternalFunctor α β] [HasExternalFunctor β α]
-           [HasExternalEquivalence α β] [HasExternalEquivalence β α] [HasInvEquiv α β]
+  variable {U V : Universe} [HasFunctoriality U V] [HasFunctoriality V U]
+           [HasEquivalenceCondition U V] [HasEquivalenceCondition V U] [HasInvEquiv U V]
 
-  def invEquiv (E : α ⟷' β) : β ⟷' α := HasExternalEquivalence.fromDefEquiv (defInvEquiv E)
+  def invEquiv' {α : U} {β : V} (E : α ⟷' β) : β ⟷' α := HasEquivalenceCondition.fromDefEquiv (defInvEquiv E)
 
 end HasInvEquiv
 
+class HasCompEquiv (U V W : Universe) [HasFunctoriality U V] [HasFunctoriality V W] [HasFunctoriality U W]
+                                      [HasFunctoriality V U] [HasFunctoriality W V] [HasFunctoriality W U]
+                   [HasEquivalenceCondition U V] [HasEquivalenceCondition V W] [HasEquivalenceCondition U W]
+                   [HasCompFun U V W] [HasCompFun W V U] where
+(defCompEquiv {α : U} {β : V} {γ : W} (E : α ⟷' β) (F : β ⟷' γ) : α ⟷'[F.toFun ⊙' E.toFun, E.invFun ⊙' F.invFun] γ)
+
+namespace HasCompEquiv
+
+  variable {U V W : Universe} [HasFunctoriality U V] [HasFunctoriality V W] [HasFunctoriality U W]
+                              [HasFunctoriality V U] [HasFunctoriality W V] [HasFunctoriality W U]
+           [HasEquivalenceCondition U V] [HasEquivalenceCondition V W] [HasEquivalenceCondition U W]
+           [HasCompFun U V W] [HasCompFun W V U] [HasCompEquiv U V W]
+
+  def compEquiv' {α : U} {β : V} {γ : W} (E : α ⟷' β) (F : β ⟷' γ) : α ⟷' γ := HasEquivalenceCondition.fromDefEquiv (defCompEquiv E F)
+
+end HasCompEquiv
 
 
-class HasEmbeddedEquivalence {U : Universe.{u}} [HasEmbeddedFunctors.{u, w} U] (α β : U) where
-[hEquiv : HasExternalEquivalence.{u, u, w, w'} α β]
-[hType  : HasEmbeddedType.{u, max 1 u w w'} U (α ⟷' β)]
 
-class HasEmbeddedEquivalences (U : Universe.{u}) [HasEmbeddedFunctors.{u, w} U] where
-[hasEquiv (α β : U) : HasEmbeddedEquivalence.{u, w, w'} α β]
+class HasEquivalences (U : Universe.{u}) (V : Universe.{v}) (W : outParam Universe.{w})
+                      [HasFunctoriality.{u, v, w'} U V] [HasFunctoriality.{v, u, w'} V U]
+  extends HasEquivalenceCondition.{u, v, w', w''} U V where
+[embed (α : U) (β : V) : HasEmbeddedType.{w, max 1 u v w' w''} W (α ⟷' β)]
 
-namespace HasEmbeddedEquivalences
+namespace HasEquivalences
 
-  variable {U : Universe} [HasEmbeddedFunctors U] [h : HasEmbeddedEquivalences U]
+  variable {U V W X Y : Universe} [HasFunctors U V X] [HasFunctors V U Y] [h : HasEquivalences U V W]
 
-  instance hasExternalEquivalence (α β : U) : HasExternalEquivalence α β := (h.hasEquiv α β).hEquiv
-  instance hasEmbeddedType        (α β : U) : HasEmbeddedType U (α ⟷' β) := (h.hasEquiv α β).hType
+  instance hasEmbeddedType (α : U) (β : V) : HasEmbeddedType W (α ⟷' β) := h.embed α β
 
-  def DefEquiv (α β : U) (toFun : α ⟶ β) (invFun : β ⟶ α) :=
-  HasExternalEquivalence.DefEquiv α β (HasEmbeddedFunctors.toExternal toFun) (HasEmbeddedFunctors.toExternal invFun)
+  def DefEquiv (α : U) (β : V) (toFun : α ⟶ β) (invFun : β ⟶ α) :=
+  HasEquivalenceCondition.DefEquiv α β (HasFunctors.toExternal toFun) (HasFunctors.toExternal invFun)
 
-  notation:20 α:21 " ⟷[" toFun:0 "," invFun:0 "] " β:21 => HasEmbeddedEquivalences.DefEquiv α β toFun invFun
+  notation:20 α:21 " ⟷[" toFun:0 "," invFun:0 "] " β:21 => HasEquivalences.DefEquiv α β toFun invFun
 
-  def Equiv (α β : U) : U := HasEmbeddedType.EmbeddedType U (α ⟷' β)
-  infix:20 " ⟷ " => HasEmbeddedEquivalences.Equiv
+  def Equiv (α : U) (β : V) : W := HasEmbeddedType.EmbeddedType W (α ⟷' β)
+  infix:20 " ⟷ " => HasEquivalences.Equiv
 
-  variable {α β : U}
+  variable {α : U} {β : V}
 
-  def toExternal   (E : α ⟷  β) : α ⟷' β := HasEmbeddedType.toExternal   U E
-  def fromExternal (E : α ⟷' β) : α ⟷  β := HasEmbeddedType.fromExternal U E
+  def toExternal   (E : α ⟷  β) : α ⟷' β := HasEmbeddedType.toExternal   W E
+  def fromExternal (E : α ⟷' β) : α ⟷  β := HasEmbeddedType.fromExternal W E
 
-  @[simp] theorem fromToExternal (E : α ⟷  β) : fromExternal (toExternal E) = E := HasEmbeddedType.fromToExternal U E
-  @[simp] theorem toFromExternal (E : α ⟷' β) : toExternal (fromExternal E) = E := HasEmbeddedType.toFromExternal U E
+  @[simp] theorem fromToExternal (E : α ⟷  β) : fromExternal (toExternal E) = E := HasEmbeddedType.fromToExternal W E
+  @[simp] theorem toFromExternal (E : α ⟷' β) : toExternal (fromExternal E) = E := HasEmbeddedType.toFromExternal W E
 
   def to  (E : α ⟷ β) (a : α) : β := (toExternal E).toFun  a
   def inv (E : α ⟷ β) (b : β) : α := (toExternal E).invFun b
 
-  def toFun  (E : α ⟷ β) : α ⟶ β := HasEmbeddedFunctors.fromExternal (toExternal E).toFun
-  def invFun (E : α ⟷ β) : β ⟶ α := HasEmbeddedFunctors.fromExternal (toExternal E).invFun
+  def toFun  (E : α ⟷ β) : α ⟶ β := HasFunctors.fromExternal (toExternal E).toFun
+  def invFun (E : α ⟷ β) : β ⟶ α := HasFunctors.fromExternal (toExternal E).invFun
 
   @[simp] theorem toFun.eff  (E : α ⟷ β) (a : α) : (toFun  E) a = to  E a :=
-  by apply HasEmbeddedFunctors.fromExternal.eff
+  by apply HasFunctors.fromExternal.eff
   @[simp] theorem invFun.eff (E : α ⟷ β) (b : β) : (invFun E) b = inv E b :=
-  by apply HasEmbeddedFunctors.fromExternal.eff
+  by apply HasFunctors.fromExternal.eff
 
-  @[simp] theorem toFun.extern  (E : α ⟷ β) : HasEmbeddedFunctors.toExternal (toFun E)  = (toExternal E).toFun :=
-  HasEmbeddedFunctors.toFromExternal (toExternal E).toFun
-  @[simp] theorem invFun.extern (E : α ⟷ β) : HasEmbeddedFunctors.toExternal (invFun E) = (toExternal E).invFun :=
-  HasEmbeddedFunctors.toFromExternal (toExternal E).invFun
+  @[simp] theorem toFun.extern  (E : α ⟷ β) : HasFunctors.toExternal (toFun E)  = (toExternal E).toFun :=
+  HasFunctors.toFromExternal (toExternal E).toFun
+  @[simp] theorem invFun.extern (E : α ⟷ β) : HasFunctors.toExternal (invFun E) = (toExternal E).invFun :=
+  HasFunctors.toFromExternal (toExternal E).invFun
 
   @[simp] theorem toFromExternal.to  (E : α ⟷' β) : (toExternal (fromExternal E)).toFun  = E.toFun  :=
-  congrArg HasExternalEquivalence.Equiv.toFun  (toFromExternal E)
+  congrArg HasEquivalenceCondition.Equiv.toFun  (toFromExternal E)
   @[simp] theorem toFromExternal.inv (E : α ⟷' β) : (toExternal (fromExternal E)).invFun = E.invFun :=
-  congrArg HasExternalEquivalence.Equiv.invFun (toFromExternal E)
+  congrArg HasEquivalenceCondition.Equiv.invFun (toFromExternal E)
 
   @[simp] theorem fromExternal.to.eff  (E : α ⟷' β) (a : α) : to  (fromExternal E) a = E.toFun  a :=
-  congrFun (congrArg HasExternalFunctor.Fun.f (toFromExternal.to  E)) a
+  congrFun (congrArg HasFunctoriality.Fun.f (toFromExternal.to  E)) a
   @[simp] theorem fromExternal.inv.eff (E : α ⟷' β) (b : β) : inv (fromExternal E) b = E.invFun b :=
-  congrFun (congrArg HasExternalFunctor.Fun.f (toFromExternal.inv E)) b
+  congrFun (congrArg HasFunctoriality.Fun.f (toFromExternal.inv E)) b
 
   def fromDefEquiv {to : α ⟶ β} {inv : β ⟶ α} (E : α ⟷[to,inv] β) : α ⟷ β :=
-  fromExternal (HasExternalEquivalence.fromDefEquiv E)
+  fromExternal (HasEquivalenceCondition.fromDefEquiv E)
 
   instance {to : α ⟶ β} {inv : β ⟶ α} : Coe (α ⟷[to,inv] β) ⌈α ⟷ β⌉ := ⟨fromDefEquiv⟩
 
   @[simp] theorem fromDefEquiv.to.eff  {to : α ⟶ β} {inv : β ⟶ α} (E : α ⟷[to,inv] β) :
     toFun  (fromDefEquiv E) = to  :=
-  by simp [fromDefEquiv, toFun,  HasExternalEquivalence.fromDefEquiv]
+  by simp [fromDefEquiv, toFun,  HasEquivalenceCondition.fromDefEquiv]
   @[simp] theorem fromDefEquiv.inv.eff {to : α ⟶ β} {inv : β ⟶ α} (E : α ⟷[to,inv] β) :
     invFun (fromDefEquiv E) = inv :=
-  by simp [fromDefEquiv, invFun, HasExternalEquivalence.fromDefEquiv]
+  by simp [fromDefEquiv, invFun, HasEquivalenceCondition.fromDefEquiv]
+
+end HasEquivalences
+
+
+
+class HasEmbeddedEquivalences (U : Universe.{u}) [HasEmbeddedFunctors.{u, w} U] [HasEmbeddedProducts.{u} U]
+  extends HasEquivalences.{u, u, u, w, w'} U U U where
+(defElimFun (α β : U) : (α ⟷ β) ⟶[λ E => HasProducts.intro (HasEquivalences.toFun E) (HasEquivalences.invFun E)] (α ⟶ β) ⊓ (β ⟶ α))
+
+namespace HasEmbeddedEquivalences
+
+  variable {U : Universe} [HasEmbeddedFunctors U] [HasEmbeddedProducts U] [HasEmbeddedEquivalences U]
+
+  @[reducible] def elimFun (α β : U) : (α ⟷ β) ⟶ (α ⟶ β) ⊓ (β ⟶ α) := defElimFun α β
 
 end HasEmbeddedEquivalences
 
 
 
-class HasFunctorialEquivalences (U : Universe.{u}) [HasEmbeddedFunctors.{u, w} U] [HasEmbeddedProducts.{u} U]
-  extends HasEmbeddedEquivalences.{u, w, w'} U where
-(defElimFun (α β : U) : (α ⟷ β) ⟶[λ E => HasEmbeddedProducts.intro (HasEmbeddedEquivalences.toFun E) (HasEmbeddedEquivalences.invFun E)] (α ⟶ β) ⊓ (β ⟶ α))
-
-namespace HasFunctorialEquivalences
-
-  variable {U : Universe} [HasEmbeddedFunctors U] [HasEmbeddedProducts U] [HasFunctorialEquivalences U]
-
-  @[reducible] def elimFun (α β : U) : (α ⟷ β) ⟶ (α ⟶ β) ⊓ (β ⟶ α) := defElimFun α β
-
-end HasFunctorialEquivalences
-
-
-
 class HasEquivOp (U : Universe.{u}) [HasEmbeddedFunctors.{u, w} U] [HasEmbeddedProducts.{u} U] [HasLinearFunOp U]
-  extends HasFunctorialEquivalences.{u, w, w'} U where
+  extends HasEmbeddedEquivalences.{u, w, w'} U where
 (defIdEquiv         (α : U)                             : α ⟷[HasLinearFunOp.idFun α, HasLinearFunOp.idFun α] α)
-(defCompEquiv       {α β γ : U} (E : α ⟷ β) (F : β ⟷ γ) : α ⟷[HasEmbeddedEquivalences.toFun F ⊙ HasEmbeddedEquivalences.toFun E, HasEmbeddedEquivalences.invFun E ⊙ HasEmbeddedEquivalences.invFun F] γ)
+(defCompEquiv       {α β γ : U} (E : α ⟷ β) (F : β ⟷ γ) : α ⟷[HasEquivalences.toFun F ⊙ HasEquivalences.toFun E, HasEquivalences.invFun E ⊙ HasEquivalences.invFun F] γ)
 (defCompEquivFun    {α β : U} (E : α ⟷ β) (γ : U)       : (β ⟷ γ) ⟶[λ F => defCompEquiv E F] (α ⟷ γ))
 (defCompEquivFunFun (α β γ : U)                         : (α ⟷ β) ⟶[λ E => defCompEquivFun E γ] ((β ⟷ γ) ⟶ (α ⟷ γ)))
-(defInvEquiv        {α β : U} (E : α ⟷ β)               : β ⟷[HasEmbeddedEquivalences.invFun E, HasEmbeddedEquivalences.toFun E] α)
+(defInvEquiv        {α β : U} (E : α ⟷ β)               : β ⟷[HasEquivalences.invFun E, HasEquivalences.toFun E] α)
 (defInvEquivFun     (α β : U)                           : (α ⟷ β) ⟶[λ E => defInvEquiv E] (β ⟷ α))
 
 namespace HasEquivOp
 
   variable {U : Universe.{u}} [HasEmbeddedFunctors U] [HasEmbeddedProducts U] [HasLinearFunOp U] [HasEquivOp U]
 
-  instance (α : U) : HasIdEquiv α := ⟨HasEmbeddedFunctors.toFromExternal (HasIdFun.idFun α) ▸ defIdEquiv α⟩
+  instance hasIdEquiv : HasIdEquiv U := ⟨λ α => HasFunctors.toFromExternal (HasIdFun.idFun' α) ▸ defIdEquiv α⟩
 
   @[reducible] def idEquiv (α : U) : α ⟷ α := defIdEquiv α
 
   -- TODO
-  --instance (α β γ : U) : HasCompEquiv α β γ :=
-  --⟨λ E F => HasEmbeddedFunctors.toFromExternal (F.toFun  ⊙' E.toFun)  ▸
-  --          HasEmbeddedFunctors.toFromExternal (E.invFun ⊙' F.invFun) ▸
-  --          HasEmbeddedEquivalences.toFromExternal E ▸
-  --          HasEmbeddedEquivalences.toFromExternal F ▸
-  --          defCompEquiv (HasEmbeddedEquivalences.fromExternal E) (HasEmbeddedEquivalences.fromExternal F)⟩
+  --instance hasCompEquiv : HasCompEquiv U U U :=
+  --⟨λ E F => HasFunctors.toFromExternal (F.toFun  ⊙' E.toFun)  ▸
+  --          HasFunctors.toFromExternal (E.invFun ⊙' F.invFun) ▸
+  --          HasEquivalences.toFromExternal E ▸
+  --          HasEquivalences.toFromExternal F ▸
+  --          defCompEquiv (HasEquivalences.fromExternal E) (HasEquivalences.fromExternal F)⟩
 
   @[reducible] def compEquiv {α β γ : U} (E : α ⟷ β) (F : β ⟷ γ) : α ⟷ γ := defCompEquiv E F
   @[reducible] def compEquivFun {α β : U} (E : α ⟷ β) (γ : U) : (β ⟷ γ) ⟶ (α ⟷ γ) := defCompEquivFun E γ
   @[reducible] def compEquivFunFun (α β γ : U) : (α ⟷ β) ⟶ (β ⟷ γ) ⟶ (α ⟷ γ) := defCompEquivFunFun α β γ
 
-  instance (α β : U) : HasInvEquiv α β :=
-  ⟨λ E => HasEmbeddedFunctors.toFromExternal E.invFun ▸
-          HasEmbeddedFunctors.toFromExternal E.toFun  ▸
-          HasEmbeddedEquivalences.toFromExternal E ▸
-          defInvEquiv (HasEmbeddedEquivalences.fromExternal E)⟩
+  instance hasInvEquiv : HasInvEquiv U U :=
+  ⟨λ E => HasFunctors.toFromExternal E.invFun ▸
+          HasFunctors.toFromExternal E.toFun  ▸
+          HasEquivalences.toFromExternal E ▸
+          defInvEquiv (HasEquivalences.fromExternal E)⟩
 
   @[reducible] def invEquiv {α β : U} (E : α ⟷ β) : β ⟷ α := defInvEquiv E
   @[reducible] def invEquivFun (α β : U) : (α ⟷ β) ⟶ (β ⟷ α) := defInvEquivFun α β
@@ -230,42 +227,42 @@ end HasEquivOp
 
 
 class HasLinearCommonEquivalences (U : Universe.{u}) [HasEmbeddedFunctors.{u, w} U] [HasLinearFunOp.{u, w} U]
-                                  [HasFunctorialTop.{u, w} U] [HasFunctorialProducts.{u, w} U] [HasEquivOp.{u, w, w'} U] where
+                                  [HasEmbeddedTop.{u, w} U] [HasEmbeddedProducts.{u, w} U] [HasEquivOp.{u, w, w'} U] where
 (defFunDomainEquiv      {α β : U} (E : α ⟷ β) (γ : U) :
-   (β ⟶ γ) ⟷[HasLinearFunOp.compFunFun (HasEmbeddedEquivalences.toFun  E) γ,
-             HasLinearFunOp.compFunFun (HasEmbeddedEquivalences.invFun E) γ] (α ⟶ γ))
+   (β ⟶ γ) ⟷[HasLinearFunOp.compFunFun (HasEquivalences.toFun  E) γ,
+             HasLinearFunOp.compFunFun (HasEquivalences.invFun E) γ] (α ⟶ γ))
 (defFunDomainEquivFun   (α β γ : U)                   :
    (α ⟷ β) ⟶[λ E => defFunDomainEquiv E γ] ((β ⟶ γ) ⟷ (α ⟶ γ)))
 (defFunCodomainEquiv    {α β : U} (E : α ⟷ β) (γ : U) :
-   (γ ⟶ α) ⟷[HasLinearFunOp.revCompFunFun γ (HasEmbeddedEquivalences.toFun  E),
-             HasLinearFunOp.revCompFunFun γ (HasEmbeddedEquivalences.invFun E)] (γ ⟶ β))
+   (γ ⟶ α) ⟷[HasLinearFunOp.revCompFunFun γ (HasEquivalences.toFun  E),
+             HasLinearFunOp.revCompFunFun γ (HasEquivalences.invFun E)] (γ ⟶ β))
 (defFunCodomainEquivFun (α β γ : U)                   :
    (α ⟷ β) ⟶[λ E => defFunCodomainEquiv E γ] ((γ ⟶ α) ⟷ (γ ⟶ β)))
 (defSwapFunFunEquiv     (α β γ : U)                   :
    (α ⟶ β ⟶ γ) ⟷[HasLinearFunOp.swapFunFunFun α β γ, HasLinearFunOp.swapFunFunFun β α γ] (β ⟶ α ⟶ γ))
 (defTopElimEquiv        (α : U)                       :
-   α ⟷[HasFunctorialTop.elimFunFun α,
-       HasFunctorialTop.invElimFun α] (HasEmbeddedTop.Top U ⟶ α))
+   α ⟷[HasEmbeddedTop.elimFunFun α,
+       HasEmbeddedTop.invElimFun α] (HasTop.Top U ⟶ α))
 (defProdElimFunEquiv    (α β γ : U)                   :
-   (α ⟶ β ⟶ γ) ⟷[HasFunctorialProducts.elimFunFun α β γ,
-                 HasFunctorialProducts.invElimFunFunFun α β γ] (α ⊓ β ⟶ γ))
+   (α ⟶ β ⟶ γ) ⟷[HasEmbeddedProducts.elimFunFun α β γ,
+                 HasEmbeddedProducts.invElimFunFunFun α β γ] (α ⊓ β ⟶ γ))
 (defProdFstEquiv        {α β : U} (E : α ⟷ β) (γ : U) :
-   α ⊓ γ ⟷[HasFunctorialProducts.replaceFstFun (HasEmbeddedEquivalences.toFun  E) γ,
-           HasFunctorialProducts.replaceFstFun (HasEmbeddedEquivalences.invFun E) γ] β ⊓ γ)
+   α ⊓ γ ⟷[HasEmbeddedProducts.replaceFstFun (HasEquivalences.toFun  E) γ,
+           HasEmbeddedProducts.replaceFstFun (HasEquivalences.invFun E) γ] β ⊓ γ)
 (defProdFstEquivFun     (α β γ : U)                   :
    (α ⟷ β) ⟶[λ E => defProdFstEquiv E γ] (α ⊓ γ ⟷ β ⊓ γ))
 (defProdSndEquiv        {α β : U} (E : α ⟷ β) (γ : U) :
-   γ ⊓ α ⟷[HasFunctorialProducts.replaceSndFun (HasEmbeddedEquivalences.toFun  E) γ,
-           HasFunctorialProducts.replaceSndFun (HasEmbeddedEquivalences.invFun E) γ] γ ⊓ β)
+   γ ⊓ α ⟷[HasEmbeddedProducts.replaceSndFun (HasEquivalences.toFun  E) γ,
+           HasEmbeddedProducts.replaceSndFun (HasEquivalences.invFun E) γ] γ ⊓ β)
 (defProdSndEquivFun     (α β γ : U)                   :
    (α ⟷ β) ⟶[λ E => defProdSndEquiv E γ] (γ ⊓ α ⟷ γ ⊓ β))
 (defProdCommEquiv       (α β : U)                     :
-   α ⊓ β ⟷[HasFunctorialProducts.commFun α β, HasFunctorialProducts.commFun β α] β ⊓ α)
+   α ⊓ β ⟷[HasEmbeddedProducts.commFun α β, HasEmbeddedProducts.commFun β α] β ⊓ α)
 (defProdAssocEquiv      (α β γ : U)                   :
-   (α ⊓ β) ⊓ γ ⟷[HasFunctorialProducts.assocLRFun α β γ, HasFunctorialProducts.assocRLFun α β γ] α ⊓ (β ⊓ γ))
+   (α ⊓ β) ⊓ γ ⟷[HasEmbeddedProducts.assocLRFun α β γ, HasEmbeddedProducts.assocRLFun α β γ] α ⊓ (β ⊓ γ))
 (defProdTopEquiv        (α : U)                       :
-   α ⟷[HasFunctorialProducts.prodTopIntroFun α,
-       HasFunctorialProducts.prodTopElimFun α] HasEmbeddedTop.Top U ⊓ α)
+   α ⟷[HasEmbeddedProducts.prodTopIntroFun α,
+       HasEmbeddedProducts.prodTopElimFun α] HasTop.Top U ⊓ α)
 (defCompEquivEquiv      {α β : U} (E : α ⟷ β) (γ : U) :
    (β ⟷ γ) ⟷[HasEquivOp.compEquivFun E γ, HasEquivOp.compEquivFun (HasEquivOp.invEquiv E) γ] (α ⟷ γ))
 (defCompEquivEquivFun   (α β γ : U)                   :
@@ -275,8 +272,8 @@ class HasLinearCommonEquivalences (U : Universe.{u}) [HasEmbeddedFunctors.{u, w}
 
 namespace HasLinearCommonEquivalences
 
-  variable {U : Universe.{u}} [HasEmbeddedFunctors U] [HasLinearFunOp U] [HasFunctorialTop U]
-           [HasFunctorialProducts U] [HasEquivOp U] [HasLinearCommonEquivalences U]
+  variable {U : Universe.{u}} [HasEmbeddedFunctors U] [HasLinearFunOp U] [HasEmbeddedTop U]
+           [HasEmbeddedProducts U] [HasEquivOp U] [HasLinearCommonEquivalences U]
 
   @[reducible] def funDomainEquiv {α β : U} (E : α ⟷ β) (γ : U) : (β ⟶ γ) ⟷ (α ⟶ γ) := defFunDomainEquiv E γ
   @[reducible] def funDomainEquivFun (α β γ : U) : (α ⟷ β) ⟶ ((β ⟶ γ) ⟷ (α ⟶ γ)) := defFunDomainEquivFun α β γ
@@ -284,7 +281,7 @@ namespace HasLinearCommonEquivalences
   @[reducible] def funCodomainEquivFun (α β γ : U) : (α ⟷ β) ⟶ ((γ ⟶ α) ⟷ (γ ⟶ β)) := defFunCodomainEquivFun α β γ
   @[reducible] def swapFunFunEquiv (α β γ : U) : (α ⟶ β ⟶ γ) ⟷ (β ⟶ α ⟶ γ) := defSwapFunFunEquiv α β γ
 
-  @[reducible] def topElimEquiv (α : U) : α ⟷ (HasEmbeddedTop.Top U ⟶ α) := defTopElimEquiv α
+  @[reducible] def topElimEquiv (α : U) : α ⟷ (HasTop.Top U ⟶ α) := defTopElimEquiv α
 
   @[reducible] def prodElimFunEquiv (α β γ : U) : (α ⟶ β ⟶ γ) ⟷ (α ⊓ β ⟶ γ) := defProdElimFunEquiv α β γ
   @[reducible] def prodFstEquiv {α β : U} (E : α ⟷ β) (γ : U) : α ⊓ γ ⟷ β ⊓ γ := defProdFstEquiv E γ
@@ -293,7 +290,7 @@ namespace HasLinearCommonEquivalences
   @[reducible] def prodSndEquivFun (α β γ : U) : (α ⟷ β) ⟶ (γ ⊓ α ⟷ γ ⊓ β) := defProdSndEquivFun α β γ
   @[reducible] def prodCommEquiv (α β : U) : α ⊓ β ⟷ β ⊓ α := defProdCommEquiv α β
   @[reducible] def prodAssocEquiv (α β γ : U) : (α ⊓ β) ⊓ γ ⟷ α ⊓ (β ⊓ γ) := defProdAssocEquiv α β γ
-  @[reducible] def prodTopEquiv (α : U) : α ⟷ HasEmbeddedTop.Top U ⊓ α := defProdTopEquiv α
+  @[reducible] def prodTopEquiv (α : U) : α ⟷ HasTop.Top U ⊓ α := defProdTopEquiv α
 
   @[reducible] def compEquivEquiv {α β : U} (E : α ⟷ β) (γ : U) : (β ⟷ γ) ⟷ (α ⟷ γ) := defCompEquivEquiv E γ
   @[reducible] def compEquivEquivFun (α β γ : U) : (α ⟷ β) ⟶ ((β ⟷ γ) ⟷ (α ⟷ γ)) := defCompEquivEquivFun α β γ
@@ -301,15 +298,15 @@ namespace HasLinearCommonEquivalences
 
 end HasLinearCommonEquivalences
 
-class HasNonLinearCommonEquivalences (U : Universe.{u}) [HasFunOp.{u, w} U] [HasFunctorialTop.{u, w} U]
-                                     [HasFunctorialProducts.{u} U] [HasEquivOp.{u, w, w'} U] where
+class HasNonLinearCommonEquivalences (U : Universe.{u}) [HasFunOp.{u, w} U] [HasEmbeddedTop.{u, w} U]
+                                     [HasEmbeddedProducts.{u} U] [HasEquivOp.{u, w, w'} U] where
 (defProdDistrEquiv (α β γ : U) :
-   (α ⟶ β ⊓ γ) ⟷[HasFunctorialProducts.distrFun α β γ,
-                 HasFunctorialProducts.invDistrFunFun α β γ] (α ⟶ β) ⊓ (α ⟶ γ))
+   (α ⟶ β ⊓ γ) ⟷[HasEmbeddedProducts.distrFun α β γ,
+                 HasEmbeddedProducts.invDistrFunFun α β γ] (α ⟶ β) ⊓ (α ⟶ γ))
 
 namespace HasNonLinearCommonEquivalences
 
-  variable {U : Universe.{u}} [HasFunOp U] [HasFunctorialTop U] [HasFunctorialProducts U]
+  variable {U : Universe.{u}} [HasFunOp U] [HasEmbeddedTop U] [HasEmbeddedProducts U]
            [HasEquivOp U] [HasNonLinearCommonEquivalences U]
 
   @[reducible] def prodDistrEquiv (α β γ : U) : (α ⟶ β ⊓ γ) ⟷ (α ⟶ β) ⊓ (α ⟶ γ):= defProdDistrEquiv α β γ
@@ -317,41 +314,41 @@ namespace HasNonLinearCommonEquivalences
 end HasNonLinearCommonEquivalences
 
 class HasBotEquivalences (U : Universe.{u}) [HasEmbeddedFunctors.{u, w} U] [HasAffineFunOp.{u, w} U]
-                         [HasFunctorialTop.{u, w} U] [HasFunctorialBot.{u, w} U]
-                         [HasFunctorialProducts.{u} U] [HasEquivOp.{u, w, w'} U] where
+                         [HasEmbeddedTop.{u, w} U] [HasEmbeddedBot.{u, w} U]
+                         [HasEmbeddedProducts.{u} U] [HasEquivOp.{u, w, w'} U] where
 (defBotNotTopEquiv         :
-   HasEmbeddedBot.Bot U ⟷[HasFunctorialBot.elimFun (HasFunctorialBot.Not (HasEmbeddedTop.Top U)),
-                          HasFunctorialBot.notTopIntroFun] HasFunctorialBot.Not (HasEmbeddedTop.Top U))
+   HasBot.Bot U ⟷[HasEmbeddedBot.elimFun (HasEmbeddedBot.Not (HasTop.Top U)),
+                  HasEmbeddedBot.notTopIntroFun] HasEmbeddedBot.Not (HasTop.Top U))
 (defProdBotEquiv   (α : U) :
-   HasEmbeddedBot.Bot U ⟷[HasFunctorialBot.elimFun (HasEmbeddedBot.Bot U ⊓ α),
-                          HasFunctorialProducts.fstFun (HasEmbeddedBot.Bot U) α] HasEmbeddedBot.Bot U ⊓ α)
+   HasBot.Bot U ⟷[HasEmbeddedBot.elimFun (HasBot.Bot U ⊓ α),
+                  HasEmbeddedProducts.fstFun (HasBot.Bot U) α] HasBot.Bot U ⊓ α)
 (defBotContraEquiv (α : U) :
-   HasEmbeddedBot.Bot U ⟷[HasFunctorialBot.elimFun (α ⊓ HasFunctorialBot.Not α),
-                          HasFunctorialProducts.elimFun (HasFunctorialBot.contraIntroFun α)] α ⊓ HasFunctorialBot.Not α)
+   HasBot.Bot U ⟷[HasEmbeddedBot.elimFun (α ⊓ HasEmbeddedBot.Not α),
+                  HasEmbeddedProducts.elimFun (HasEmbeddedBot.contraIntroFun α)] α ⊓ HasEmbeddedBot.Not α)
 
 namespace HasBotEquivalences
 
-  variable {U : Universe.{u}} [HasEmbeddedFunctors U] [HasAffineFunOp U] [HasFunctorialTop U]
-           [HasFunctorialBot U] [HasFunctorialProducts U] [HasEquivOp U] [HasBotEquivalences U]
+  variable {U : Universe.{u}} [HasEmbeddedFunctors U] [HasAffineFunOp U] [HasEmbeddedTop U]
+           [HasEmbeddedBot U] [HasEmbeddedProducts U] [HasEquivOp U] [HasBotEquivalences U]
 
-  @[reducible] def botNotTopEquiv : HasEmbeddedBot.Bot U ⟷ HasFunctorialBot.Not (HasEmbeddedTop.Top U) := defBotNotTopEquiv (U := U)
-  @[reducible] def prodBotEquiv (α : U) : HasEmbeddedBot.Bot U ⟷ HasEmbeddedBot.Bot U ⊓ α := defProdBotEquiv α
-  @[reducible] def botContraEquiv (α : U) : HasEmbeddedBot.Bot U ⟷ α ⊓ HasFunctorialBot.Not α := defBotContraEquiv α
+  @[reducible] def botNotTopEquiv : HasBot.Bot U ⟷ HasEmbeddedBot.Not (HasTop.Top U) := defBotNotTopEquiv (U := U)
+  @[reducible] def prodBotEquiv (α : U) : HasBot.Bot U ⟷ HasBot.Bot U ⊓ α := defProdBotEquiv α
+  @[reducible] def botContraEquiv (α : U) : HasBot.Bot U ⟷ α ⊓ HasEmbeddedBot.Not α := defBotContraEquiv α
 
 end HasBotEquivalences
 
 class HasClassicalEquivalences (U : Universe.{u}) [HasEmbeddedFunctors.{u, w} U] [HasLinearFunOp.{u, w} U]
-                               [HasFunctorialBot.{u, w} U] [HasClassicalLogic.{u, w} U]
-                               [HasFunctorialProducts.{u} U] [HasEquivOp.{u, w, w'} U] where
+                               [HasEmbeddedBot.{u, w} U] [HasClassicalLogic.{u, w} U]
+                               [HasEmbeddedProducts.{u} U] [HasEquivOp.{u, w, w'} U] where
 (defByContradictionEquiv (α : U) :
-   α ⟷[HasFunctorialBot.notNotFun α,
-       HasClassicalLogic.byContradictionFun α] HasFunctorialBot.Not (HasFunctorialBot.Not α))
+   α ⟷[HasEmbeddedBot.notNotFun α,
+       HasClassicalLogic.byContradictionFun α] HasEmbeddedBot.Not (HasEmbeddedBot.Not α))
 
 namespace HasClassicalEquivalences
 
-  variable {U : Universe.{u}} [HasEmbeddedFunctors U] [HasLinearFunOp U] [HasFunctorialBot U]
-           [HasClassicalLogic U] [HasFunctorialProducts U] [HasEquivOp U] [HasClassicalEquivalences U]
+  variable {U : Universe.{u}} [HasEmbeddedFunctors U] [HasLinearFunOp U] [HasEmbeddedBot U]
+           [HasClassicalLogic U] [HasEmbeddedProducts U] [HasEquivOp U] [HasClassicalEquivalences U]
 
-  @[reducible] def byContradictionEquiv (α : U) : α ⟷ HasFunctorialBot.Not (HasFunctorialBot.Not α) := defByContradictionEquiv α
+  @[reducible] def byContradictionEquiv (α : U) : α ⟷ HasEmbeddedBot.Not (HasEmbeddedBot.Not α) := defByContradictionEquiv α
 
 end HasClassicalEquivalences
