UniverseAbstractions/Axioms/Universe/Functors.lean
@@ -5,7 +5,7 @@ import UniverseAbstractions.Axioms.Universes
 set_option autoBoundImplicitLocal false
 --set_option pp.universes true
 
-universe u v w
+universe u v w w'
 
 
 
@@ -16,7 +16,7 @@ universe u v w
 --   define e.g. functors returning functors without having to specify any additional assumptions.
 --   E.g. if `U` is the universe of categories, `α ⟶ β` is the functor category from `α` to `β`.
 --
--- * However, in some cases we have a more general concept of a functor `α ⟶' β` where `α` and `β`
+-- * However, in some cases we have a more general concept of a functor `α ⟶ β` where `α` and `β`
 --   are not necessarily types of the same universe.
 --
 -- * Moreover, we want to axiomatically assert the existence of certain functors such as identity
@@ -27,34 +27,34 @@ universe u v w
 -- In order to meet all requirements, we currently define three kinds of functors, with conversions
 -- between them:
 --
--- `α : U`, `β : V` | `F : α ⟶[f] β` | `F a` defined as `f a`.
---                  | `F : α ⟶' β`   | Bundled version of the above; therefore e.g. `(idFun α) a`
---                  |                | (see below) is definitionally equal to `a`.
--- `α β : U`        | `F : α ⟶ β`    | An instance of `U`; therefore `F a` cannot be definitionally
---                  |                | equal to anything if `U` is arbitrary. In particular, e.g.
---                  |                | `(idFun α) a = a` not definitionally, but `by simp` (more
---                  |                | specifically, `fromDefFun.eff`).
+-- `F : α ⟶[f] β` | `F a` defined as `f a`.
+-- `F : α ⟶' β`   | Bundled version of the above; therefore e.g. `(HasIdFun.idFun α) a` (see below)
+--                | is definitionally equal to `a`.
+-- `F : α ⟶ β`    | An instance of a universe `W`; therefore we cannot ensure that `F a` is
+--                | definitionally equal to anything if `W` is arbitrary.
+--                | In particular, e.g. `(HasLinearFunOp.idFun α) a = a` not definitionally, but
+--                | `by simp` (more specifically, `HasFunctor.fromDefFun.eff`).
 
 
 
-class HasExternalFunctor {U : Universe.{u}} {V : Universe.{v}} (α : U) (β : V) : Sort (max u v (w + 1)) where
-(IsFun : (α → β) → Sort w)
+class HasFunctoriality (U : Universe.{u}) (V : Universe.{v}) : Type (max u v w) where
+(IsFun {α : U} {β : V} : (α → β) → Sort w)
 
-namespace HasExternalFunctor
+namespace HasFunctoriality
 
-  def DefFun {U : Universe.{u}} {V : Universe.{v}} (α : U) (β : V) [h : HasExternalFunctor.{u, v, w} α β]
+  def DefFun {U : Universe.{u}} {V : Universe.{v}} [h : HasFunctoriality.{u, v, w} U V] (α : U) (β : V)
              (f : α → β) :=
   h.IsFun f
-  notation:20 α:21 " ⟶[" f:0 "] " β:21 => HasExternalFunctor.DefFun α β f
+  notation:20 α:21 " ⟶[" f:0 "] " β:21 => HasFunctoriality.DefFun α β f
 
-  structure Fun {U : Universe.{u}} {V : Universe.{v}} (α : U) (β : V) [HasExternalFunctor.{u, v, w} α β] :
+  structure Fun {U : Universe.{u}} {V : Universe.{v}} [HasFunctoriality.{u, v, w} U V] (α : U) (β : V) :
     Sort (max 1 u v w) where
   (f : α → β)
   (F : α ⟶[f] β)
 
-  infixr:20 " ⟶' " => HasExternalFunctor.Fun
+  infixr:20 " ⟶' " => HasFunctoriality.Fun
 
-  variable {U : Universe.{u}} {V : Universe.{v}} {α : U} {β : V} [HasExternalFunctor.{u, v, w} α β]
+  variable {U : Universe.{u}} {V : Universe.{v}} [HasFunctoriality.{u, v, w} U V] {α : U} {β : V}
 
   instance coeDefFun (f : α → β) : CoeFun (α ⟶[f] β) (λ _ => α → β) := ⟨λ _ => f⟩
   instance coeFun                : CoeFun (α ⟶' β)   (λ _ => α → β) := ⟨Fun.f⟩
@@ -86,105 +86,61 @@ namespace HasExternalFunctor
   match F with | ⟨_, _⟩ => rfl
   @[simp] theorem toFromDefFun {f : α → β} (F : α ⟶[f] β) : toDefFun (fromDefFun F) = F := rfl
 
-end HasExternalFunctor
+end HasFunctoriality
 
 
 
-class HasIdFun {U : Universe} (α : U) [HasExternalFunctor α α] where
-(defIdFun : α ⟶[id] α)
+class HasFunctors (U : Universe.{u}) (V : Universe.{v}) (W : outParam Universe.{w})
+  extends HasFunctoriality.{u, v, w'} U V : Type (max u v w w') where
+[embed (α : U) (β : V) : HasEmbeddedType.{w, max 1 u v w'} W (α ⟶' β)]
 
-namespace HasIdFun
+namespace HasFunctors
 
-  variable {U : Universe} (α : U) [HasExternalFunctor α α] [HasIdFun α]
+  variable {U V W : Universe} [h : HasFunctors U V W]
 
-  def idFun : α ⟶' α := HasExternalFunctor.fromDefFun defIdFun
+  instance hasEmbeddedType (α : U) (β : V) : HasEmbeddedType W (α ⟶' β) := h.embed α β
 
-end HasIdFun
+  @[reducible] def DefFun (α : U) (β : V) (f : α → β) := HasFunctoriality.DefFun α β f
 
-class HasConstFun {U V : Universe} (α : U) (β : V) [HasExternalFunctor α β] where
-(defConstFun (c : β) : α ⟶[Function.const ⌈α⌉ c] β)
+  def Fun (α : U) (β : V) : W := HasEmbeddedType.EmbeddedType W (α ⟶' β)
+  infixr:20 " ⟶ " => HasFunctors.Fun
 
-namespace HasConstFun
+  variable {α : U} {β : V}
 
-  variable {U V : Universe} (α : U) {β : V} [HasExternalFunctor α β] [HasConstFun α β]
-
-  def constFun (c : β) : α ⟶' β := HasExternalFunctor.fromDefFun (defConstFun c)
-
-end HasConstFun
-
-class HasCompFun {U V W : Universe} (α : U) (β : V) (γ : W)
-                 [HasExternalFunctor α β] [HasExternalFunctor β γ] [HasExternalFunctor α γ] where
-(defCompFun (F : α ⟶' β) (G : β ⟶' γ) : α ⟶[λ a => G (F a)] γ)
-
-namespace HasCompFun
-
-  variable {U V W : Universe} {α : U} {β : V} {γ : W}
-           [HasExternalFunctor α β] [HasExternalFunctor β γ] [HasExternalFunctor α γ] [HasCompFun α β γ]
-
-  def compFun (F : α ⟶' β) (G : β ⟶' γ) : α ⟶' γ := HasExternalFunctor.fromDefFun (defCompFun F G)
-
-  @[reducible] def revCompFun (G : β ⟶' γ) (F : α ⟶' β) := compFun F G
-  infixr:90 " ⊙' " => HasCompFun.revCompFun
-
-end HasCompFun
-
-
-
-class HasEmbeddedFunctor {U : Universe.{u}} (α β : U) : Type (max u w) where
-[hFun  : HasExternalFunctor.{u, u, w} α β]
-[hType : HasEmbeddedType.{u, max 1 u w} U (α ⟶' β)]
-
-class HasEmbeddedFunctors (U : Universe.{u}) : Type (max u w) where
-[hasFun (α β : U) : HasEmbeddedFunctor.{u, w} α β]
-
-namespace HasEmbeddedFunctors
-
-  variable {U : Universe} [h : HasEmbeddedFunctors U]
-
-  instance hasExternalFunctor (α β : U) : HasExternalFunctor α β     := (h.hasFun α β).hFun
-  instance hasEmbeddedType    (α β : U) : HasEmbeddedType U (α ⟶' β) := (h.hasFun α β).hType
-
-  @[reducible] def DefFun (α β : U) (f : α → β) := HasExternalFunctor.DefFun α β f
-
-  def Fun (α β : U) : U := HasEmbeddedType.EmbeddedType U (α ⟶' β)
-  infixr:20 " ⟶ " => HasEmbeddedFunctors.Fun
-
-  variable {α β : U}
-
-  def toExternal   (F : α ⟶  β) : α ⟶' β := HasEmbeddedType.toExternal   U F
-  def fromExternal (F : α ⟶' β) : α ⟶  β := HasEmbeddedType.fromExternal U F
+  def toExternal   (F : α ⟶  β) : α ⟶' β := HasEmbeddedType.toExternal   W F
+  def fromExternal (F : α ⟶' β) : α ⟶  β := HasEmbeddedType.fromExternal W F
 
   def funCoe (F : α ⟶ β) : α → β := (toExternal F).f
   instance coeFun : CoeFun ⌈α ⟶ β⌉ (λ _ => α → β) := ⟨funCoe⟩
 
-  @[simp] theorem fromToExternal (F : α ⟶ β)  : fromExternal (toExternal F) = F := HasEmbeddedType.fromToExternal U F
-  @[simp] theorem toFromExternal (F : α ⟶' β) : toExternal (fromExternal F) = F := HasEmbeddedType.toFromExternal U F
+  @[simp] theorem fromToExternal (F : α ⟶  β) : fromExternal (toExternal F) = F := HasEmbeddedType.fromToExternal W F
+  @[simp] theorem toFromExternal (F : α ⟶' β) : toExternal (fromExternal F) = F := HasEmbeddedType.toFromExternal W F
 
-  @[simp] theorem toExternal.eff   (F : α ⟶ β)  (a : α) : (toExternal   F) a = F a := rfl
+  @[simp] theorem toExternal.eff   (F : α ⟶  β) (a : α) : (toExternal   F) a = F a := rfl
   @[simp] theorem fromExternal.eff (F : α ⟶' β) (a : α) : (fromExternal F) a = F a :=
-  congrFun (congrArg HasExternalFunctor.Fun.f (toFromExternal F)) a
+  congrFun (congrArg HasFunctoriality.Fun.f (toFromExternal F)) a
 
   instance coeDefFun (f : α → β) : CoeFun (α ⟶[f] β) (λ _ => α → β) := ⟨λ _ => f⟩
 
-  def toDefFun               (F : α ⟶ β)    : α ⟶[funCoe F] β := HasExternalFunctor.toDefFun (toExternal F)
-  def fromDefFun {f : α → β} (F : α ⟶[f] β) : α ⟶ β           := fromExternal (HasExternalFunctor.fromDefFun F)
+  def toDefFun               (F : α ⟶ β)    : α ⟶[funCoe F] β := HasFunctoriality.toDefFun (toExternal F)
+  def fromDefFun {f : α → β} (F : α ⟶[f] β) : α ⟶ β           := fromExternal (HasFunctoriality.fromDefFun F)
 
   instance {f : α → β} : Coe (α ⟶[f] β) ⌈α ⟶ β⌉ := ⟨fromDefFun⟩
 
   def castDefFun {f f' : α → β} (F : α ⟶[f] β) (h : ∀ a, f a = f' a) : α ⟶[f'] β :=
-  HasExternalFunctor.castDefFun F h
+  HasFunctoriality.castDefFun F h
 
   @[simp] theorem fromCastDefFun {f f' : α → β} (F : α ⟶[f] β) (h : ∀ a, f a = f' a) :
     fromDefFun (castDefFun F h) = fromDefFun F :=
-  congrArg fromExternal (HasExternalFunctor.fromCastDefFun F h)
+  congrArg fromExternal (HasFunctoriality.fromCastDefFun F h)
 
   @[simp] theorem castCastDefFun {f f' : α → β} (F : α ⟶[f] β) (h : ∀ a, f a = f' a) :
     castDefFun (castDefFun F h) (λ a => Eq.symm (h a)) = F :=
-  HasExternalFunctor.castCastDefFun F h
+  HasFunctoriality.castCastDefFun F h
 
   def toDefFun' (F : α ⟶ β) {f : α → β} (h : ∀ a, F a = f a) : α ⟶[f] β :=
   castDefFun (toDefFun F) h
-  infix:60 " ◄ " => HasEmbeddedFunctors.toDefFun'
+  infix:60 " ◄ " => HasFunctors.toDefFun'
 
   -- Marking this `@[simp]` causes a huge performance hit. I don't understand why.
   theorem toDefFun'.eff (F : α ⟶ β) {f : α → β} (h : ∀ a, F a = f a) (a : α) : (toDefFun' F h) a = F a :=
@@ -192,16 +148,95 @@ namespace HasEmbeddedFunctors
 
   @[simp] theorem toDefFun.eff               (F : α ⟶ β)    (a : α) : (toDefFun   F) a = F a := rfl
   @[simp] theorem fromDefFun.eff {f : α → β} (F : α ⟶[f] β) (a : α) : (fromDefFun F) a = F a :=
-  fromExternal.eff (HasExternalFunctor.fromDefFun F) a
+  fromExternal.eff (HasFunctoriality.fromDefFun F) a
 
   @[simp] theorem fromToDefFun (F : α ⟶ β) : fromDefFun (toDefFun F) = F :=
-  Eq.trans (congrArg fromExternal (HasExternalFunctor.fromToDefFun (toExternal F))) (fromToExternal F)
+  Eq.trans (congrArg fromExternal (HasFunctoriality.fromToDefFun (toExternal F))) (fromToExternal F)
 
   @[simp] theorem fromToDefFun' (F : α ⟶ β) {f : α → β} (h : ∀ a, F a = f a) : fromDefFun (toDefFun' F h) = F :=
   Eq.trans (fromCastDefFun (toDefFun F) h) (fromToDefFun F)
 
   -- This is annoying to prove, and we don't need it at the moment.
   --@[simp] theorem toFromDefFun' {f : α → β} (F : α ⟶[f] β) : toDefFun' (fromDefFun F) (fromDefFun.eff F) = F := sorry
+
+end HasFunctors
+
+
+
+class HasIdFun (U : Universe) [HasFunctoriality U U] where
+(defIdFun (α : U) : α ⟶[id] α)
+
+namespace HasIdFun
+
+  @[reducible] def idFun' {U : Universe} [HasFunctoriality U U] [HasIdFun U] (α : U) : α ⟶' α :=
+  HasFunctoriality.fromDefFun (defIdFun α)
+
+  @[reducible] def idFun {U V : Universe} [HasFunctors U U V] [HasIdFun U] (α : U) : α ⟶ α :=
+  HasFunctors.fromExternal (idFun' α)
+
+end HasIdFun
+
+class HasConstFun (U V : Universe) [HasFunctoriality U V] where
+(defConstFun (α : U) {β : V} (c : β) : α ⟶[Function.const ⌈α⌉ c] β)
+
+namespace HasConstFun
+
+  variable {U V : Universe} [HasFunctoriality U V] [HasConstFun U V]
+
+  @[reducible] def constFun' {U V : Universe} [HasFunctoriality U V] [HasConstFun U V] (α : U) {β : V} (c : β) :
+    α ⟶' β :=
+  HasFunctoriality.fromDefFun (defConstFun α c)
+
+  @[reducible] def constFun {U V W : Universe} [HasFunctors U V W] [HasConstFun U V] (α : U) {β : V} (c : β) :
+    α ⟶ β :=
+  HasFunctors.fromExternal (constFun' α c)
+
+end HasConstFun
+
+class HasCompFun (U V W : Universe) [HasFunctoriality U V] [HasFunctoriality V W] [HasFunctoriality U W] where
+(defCompFun {α : U} {β : V} {γ : W} (F : α ⟶' β) (G : β ⟶' γ) : α ⟶[λ a => G (F a)] γ)
+
+namespace HasCompFun
+
+  @[reducible] def compFun' {U V W : Universe} [HasFunctoriality U V] [HasFunctoriality V W] [HasFunctoriality U W]
+                            [HasCompFun U V W] {α : U} {β : V} {γ : W} (F : α ⟶' β) (G : β ⟶' γ) : α ⟶' γ :=
+  HasFunctoriality.fromDefFun (defCompFun F G)
+
+  @[reducible] def revCompFun' {U V W : Universe} [HasFunctoriality U V] [HasFunctoriality V W] [HasFunctoriality U W]
+                               [HasCompFun U V W] {α : U} {β : V} {γ : W} (G : β ⟶' γ) (F : α ⟶' β) := compFun' F G
+  infixr:90 " ⊙' " => HasCompFun.revCompFun'
+
+  @[reducible] def compFun {U V W X Y Z : Universe} [HasFunctors U V X] [HasFunctors V W Y] [HasFunctors U W Z]
+                           [HasCompFun U V W] {α : U} {β : V} {γ : W} (F : α ⟶ β) (G : β ⟶ γ) : α ⟶ γ :=
+  HasFunctors.fromExternal (compFun' (HasFunctors.toExternal F) (HasFunctors.toExternal G))
+
+  @[reducible] def revCompFun {U V W X Y Z : Universe} [HasFunctors U V X] [HasFunctors V W Y] [HasFunctors U W Z]
+                              [HasCompFun U V W] {α : U} {β : V} {γ : W} (G : β ⟶ γ) (F : α ⟶ β) := compFun F G
+
+end HasCompFun
+
+
+
+class HasEmbeddedFunctors (U : Universe.{u}) extends HasFunctors.{u, u, u, w} U U U : Type (max u w)
+
+namespace HasEmbeddedFunctors
+
+  -- Restricted copies of definitions in `HasFunctors` to help functoriality tactic.
+
+  variable {U : Universe} [HasEmbeddedFunctors U]
+
+  @[reducible] def DefFun (α β : U) (f : α → β) := HasFunctors.DefFun α β f
+
+  @[reducible] def Fun (α β : U) : U := HasFunctors.Fun α β
+
+  variable {α β : U}
+
+  @[reducible] def funCoe (F : α ⟶ β) : α → β := HasFunctors.funCoe F
+
+  @[reducible] def toDefFun               (F : α ⟶ β)    : α ⟶[funCoe F] β := HasFunctors.toDefFun F
+  @[reducible] def fromDefFun {f : α → β} (F : α ⟶[f] β) : α ⟶ β           := HasFunctors.fromDefFun F
+
+  @[reducible] def toDefFun' (F : α ⟶ β) {f : α → β} (h : ∀ a, F a = f a) : α ⟶[f] β := HasFunctors.toDefFun' F h
 
 end HasEmbeddedFunctors
 
@@ -240,17 +275,16 @@ namespace HasLinearFunOp
 
   variable {U : Universe} [HasEmbeddedFunctors U] [HasLinearFunOp U]
 
-  instance (α : U) : HasIdFun α := ⟨defIdFun α⟩
+  instance hasIdFun : HasIdFun U := ⟨defIdFun⟩
 
   @[reducible] def idFun (α : U) : α ⟶ α := defIdFun α
 
   @[reducible] def appFun {α : U} (a : α) (β : U) : (α ⟶ β) ⟶ β := defAppFun a β
   @[reducible] def appFunFun (α β : U) : α ⟶ (α ⟶ β) ⟶ β := defAppFunFun α β
 
-  instance (α β γ : U) : HasCompFun α β γ :=
-  ⟨λ F G => HasEmbeddedFunctors.castDefFun (defCompFun (HasEmbeddedFunctors.fromExternal F)
-                                                       (HasEmbeddedFunctors.fromExternal G))
-                                           (λ _ => by simp)⟩
+  instance hasCompFun : HasCompFun U U U :=
+  ⟨λ F G => HasFunctors.castDefFun (defCompFun (HasFunctors.fromExternal F) (HasFunctors.fromExternal G))
+                                   (λ _ => by simp)⟩
 
   @[reducible] def compFun {α β γ : U} (F : α ⟶ β) (G : β ⟶ γ) : α ⟶ γ := defCompFun F G
   @[reducible] def compFunFun {α β : U} (F : α ⟶ β) (γ : U) : (β ⟶ γ) ⟶ (α ⟶ γ) := defCompFunFun F γ
@@ -271,7 +305,7 @@ namespace HasSubLinearFunOp
 
   variable {U : Universe} [HasEmbeddedFunctors U] [HasSubLinearFunOp U]
 
-  instance (α β : U) : HasConstFun α β := ⟨λ c => defConstFun α c⟩
+  instance hasConstFun : HasConstFun U U := ⟨defConstFun⟩
 
   @[reducible] def constFun (α : U) {β : U} (c : β) : α ⟶ β := defConstFun α c
   @[reducible] def constFunFun (α β : U) : β ⟶ (α ⟶ β) := defConstFunFun α β
