UniverseAbstractions/Axioms/Universe/Products.lean
@@ -10,66 +10,57 @@ universe u v w
 
 
 
--- The type class `HasExternalProduct` (analogously to `HasExternalFunctor` etc.) doesn't actually
--- exist because we assume that products never need to carry any additional data.
+def HasProducts.Prod {U : Universe.{u}} {V : Universe.{v}} (α : U) (β : V) := PProd ⌈α⌉ ⌈β⌉
+infix:35 " ⊓' " => HasProducts.Prod
 
-namespace HasExternalProduct
+class HasProducts (U : Universe.{u}) (V : Universe.{v}) (W : outParam Universe.{w}) where
+[embed (α : U) (β : V) : HasEmbeddedType.{w, max 1 u v} W (α ⊓' β)]
 
-  def Product {U : Universe.{u}} {V : Universe.{v}} (α : U) (β : V) := PProd ⌈α⌉ ⌈β⌉
+namespace HasProducts
 
-  infix:35 " ⊓' " => HasExternalProduct.Product
+  variable {U V W : Universe} [h : HasProducts U V W]
 
-end HasExternalProduct
+  instance hasEmbeddedType (α : U) (β : V) : HasEmbeddedType W (α ⊓' β) := h.embed α β
 
+  def Product (α : U) (β : V) : W := HasEmbeddedType.EmbeddedType W (α ⊓' β)
+  infix:35 " ⊓ " => HasProducts.Product
+  
+  variable {α : U} {β : V}
 
+  def toExternal   (P : α ⊓  β) : α ⊓' β := HasEmbeddedType.toExternal   W P
+  def fromExternal (P : α ⊓' β) : α ⊓  β := HasEmbeddedType.fromExternal W P
 
-class HasEmbeddedProduct {U : Universe.{u}} (α β : U) where
-[hType : HasEmbeddedType.{u, max 1 u} U (α ⊓' β)]
-
-class HasEmbeddedProducts (U : Universe.{u}) where
-[hasProd (α β : U) : HasEmbeddedProduct.{u} α β]
-
-namespace HasEmbeddedProducts
-
-  variable {U : Universe} [h : HasEmbeddedProducts U]
-
-  instance hasEmbeddedType (α β : U) : HasEmbeddedType U (α ⊓' β) := (h.hasProd α β).hType
-
-  def Product (α β : U) : U := HasEmbeddedType.EmbeddedType U (α ⊓' β)
-  infix:35 " ⊓ " => HasEmbeddedProducts.Product
-
-  variable {α β : U}
-
-  def toExternal   (P : α ⊓  β) : α ⊓' β := HasEmbeddedType.toExternal   U P
-  def fromExternal (P : α ⊓' β) : α ⊓  β := HasEmbeddedType.fromExternal U P
-
-  @[simp] theorem fromToExternal (P : α ⊓  β) : fromExternal (toExternal P) = P := HasEmbeddedType.fromToExternal U P
-  @[simp] theorem toFromExternal (P : α ⊓' β) : toExternal (fromExternal P) = P := HasEmbeddedType.toFromExternal U P
+  @[simp] theorem fromToExternal (P : α ⊓  β) : fromExternal (toExternal P) = P := HasEmbeddedType.fromToExternal W P
+  @[simp] theorem toFromExternal (P : α ⊓' β) : toExternal (fromExternal P) = P := HasEmbeddedType.toFromExternal W P
 
   def fst (P : α ⊓ β) : α := (toExternal P).fst
   def snd (P : α ⊓ β) : β := (toExternal P).snd
 
   def intro (a : α) (b : β) : α ⊓ β := fromExternal ⟨a, b⟩
 
-end HasEmbeddedProducts
+end HasProducts
 
 
 
--- We would like to map in and out of products functorially. Introduction is simply given by
--- `α ⟶ β ⟶ α ⊓ β`, i.e. given an `α` and a `β`, we can construct their product. For elimination,
--- we take an indirect approach that works well with `HasLinearFunOp`, `HasAffineFunOp`, and
--- `HasFullFunOp`: If only `HasLinearFunOp` is given, it is both allowed and required to always use
--- both sides of a product; eliminating to either `α` or `β` requires `constFun`.
+-- In many cases, the product of two universe instances is again an instance of the same universe.
+--
+-- Moreover, we would like to map in and out of products functorially. Introduction is simply given
+-- by `α ⟶ β ⟶ α ⊓ β`, i.e. given an `α` and a `β`, we can construct their product. For
+-- elimination, we take an indirect approach that works well with `HasLinearFunOp`,
+-- `HasAffineFunOp`, and `HasFullFunOp`: If only `HasLinearFunOp` is given, it is both allowed and
+-- required to always use both sides of a product; eliminating to either `α` or `β` requires
+-- `constFun`.
 
-class HasFunctorialProducts (U : Universe.{u}) [HasEmbeddedFunctors.{u, w} U] extends HasEmbeddedProducts U where
-(defIntroFun    {α : U} (a : α) (β : U)     : β ⟶[λ b => HasEmbeddedProducts.intro a b] α ⊓ β)
+class HasEmbeddedProducts (U : Universe.{u}) [HasEmbeddedFunctors.{u, w} U]
+  extends HasProducts.{u, u, u} U U U where
+(defIntroFun    {α : U} (a : α) (β : U)     : β ⟶[λ b => HasProducts.intro a b] α ⊓ β)
 (defIntroFunFun (α β : U)                   : α ⟶[λ a => defIntroFun a β] (β ⟶ α ⊓ β))
-(defElimFun     {α β γ : U} (F : α ⟶ β ⟶ γ) : α ⊓ β ⟶[λ P => F (HasEmbeddedProducts.fst P) (HasEmbeddedProducts.snd P)] γ)
+(defElimFun     {α β γ : U} (F : α ⟶ β ⟶ γ) : α ⊓ β ⟶[λ P => F (HasProducts.fst P) (HasProducts.snd P)] γ)
 (defElimFunFun  (α β γ : U)                 : (α ⟶ β ⟶ γ) ⟶[λ F => defElimFun F] (α ⊓ β ⟶ γ))
 
-namespace HasFunctorialProducts
+namespace HasEmbeddedProducts
 
-  variable {U : Universe} [HasEmbeddedFunctors U] [HasFunctorialProducts U]
+  variable {U : Universe} [HasEmbeddedFunctors U] [HasEmbeddedProducts U]
 
   @[reducible] def introFun {α : U} (a : α) (β : U) : β ⟶ α ⊓ β := defIntroFun a β
   @[reducible] def introFunFun (α β : U) : α ⟶ β ⟶ α ⊓ β := defIntroFunFun α β
@@ -77,4 +68,4 @@ namespace HasFunctorialProducts
   @[reducible] def elimFun {α β γ : U} (F : α ⟶ β ⟶ γ) : α ⊓ β ⟶ γ := defElimFun F
   @[reducible] def elimFunFun (α β γ : U) : (α ⟶ β ⟶ γ) ⟶ (α ⊓ β ⟶ γ) := defElimFunFun α β γ
 
-end HasFunctorialProducts
+end HasEmbeddedProducts
