UniverseAbstractions/Axioms/Universe/Singletons.lean
@@ -10,66 +10,79 @@ universe u w
 
 
 
-class HasEmbeddedTop (U : Universe.{u}) where
-[h : HasEmbeddedType.{u, 0} U True]
+class HasTop (U : Universe.{u}) where
+[embed : HasEmbeddedType.{u, 0} U True]
 
-namespace HasEmbeddedTop
+namespace HasTop
 
-  instance hasEmbeddedType (U : Universe) [h : HasEmbeddedTop U] : HasEmbeddedType U True := h.h
+  variable (U : Universe) [h : HasTop U] 
 
-  def Top (U : Universe) [HasEmbeddedTop U] : U := HasEmbeddedType.EmbeddedType U True
+  instance hasEmbeddedType : HasEmbeddedType U True := h.embed
 
-  def top (U : Universe) [HasEmbeddedTop U] : Top U := HasEmbeddedType.fromExternal U trivial
+  def Top : U := HasEmbeddedType.EmbeddedType U True
 
-end HasEmbeddedTop
+  def top : Top U := HasEmbeddedType.fromExternal U trivial
+
+end HasTop
 
 -- Eliminating from `Top` should not require `SubLinearFunOp`, as conceptually, an instance of
 -- `Top` does not hold any data. Therefore, we define a specialized version of `constFun`.
 
-class HasFunctorialTop (U : Universe.{u}) [HasEmbeddedFunctors.{u, w} U]
-  extends HasEmbeddedTop U where
-(defElimFun {α : U} (a : α) : HasEmbeddedTop.Top U ⟶[λ _ => a] α)
-(defElimFunFun (α : U) : α ⟶[λ a => defElimFun a] (HasEmbeddedTop.Top U ⟶ α))
+class HasEmbeddedTop (U : Universe.{u}) [HasEmbeddedFunctors.{u, w} U]
+  extends HasTop U where
+(defElimFun {α : U} (a : α) : HasTop.Top U ⟶[λ _ => a] α)
+(defElimFunFun (α : U) : α ⟶[λ a => defElimFun a] (HasTop.Top U ⟶ α))
 
-namespace HasFunctorialTop
+namespace HasEmbeddedTop
 
-  variable {U : Universe} [HasEmbeddedFunctors U] [HasFunctorialTop U]
+  open HasTop
 
-  @[reducible] def elimFun {α : U} (a : α) : HasEmbeddedTop.Top U ⟶ α := HasFunctorialTop.defElimFun a
-  @[reducible] def elimFunFun (α : U) : α ⟶ HasEmbeddedTop.Top U ⟶ α := defElimFunFun α
+  variable {U : Universe} [HasEmbeddedFunctors U] [HasEmbeddedTop U]
 
-end HasFunctorialTop
+  @[reducible] def elimFun {α : U} (a : α) : Top U ⟶ α := defElimFun a
+  @[reducible] def elimFunFun (α : U) : α ⟶ Top U ⟶ α := defElimFunFun α
+
+end HasEmbeddedTop
 
 
 
 
-class HasEmbeddedBot (U : Universe.{u}) where
-[h : HasEmbeddedType.{u, 0} U False]
+class HasBot (U : Universe.{u}) where
+[embed : HasEmbeddedType.{u, 0} U False]
+
+namespace HasBot
+
+  section Init
+
+    variable (U : Universe) [h : HasBot U]
+
+    instance hasEmbeddedType : HasEmbeddedType U False := h.embed
+
+    def Bot : U := HasEmbeddedType.EmbeddedType U False
+
+  end Init
+
+  variable {U : Universe} [h : HasBot U]
+
+  def elim (e : Bot U) {α : U} : α := False.elim (HasEmbeddedType.toExternal U e)
+
+end HasBot
+
+class HasEmbeddedBot (U : Universe.{u}) [HasEmbeddedFunctors.{u, w} U]
+  extends HasBot U where
+(defElimFun (α : U) : HasBot.Bot U ⟶[λ e => HasBot.elim e] α)
 
 namespace HasEmbeddedBot
 
-  instance hasEmbeddedType (U : Universe) [h : HasEmbeddedBot U] : HasEmbeddedType U False := h.h
+  open HasBot
 
-  def Bot (U : Universe) [h : HasEmbeddedBot U] : U := HasEmbeddedType.EmbeddedType U False
+  variable {U : Universe} [HasEmbeddedFunctors U] [HasEmbeddedBot U]
 
-  def elim {U : Universe} [h : HasEmbeddedBot U] (e : Bot U) {α : U} : α :=
-  False.elim (HasEmbeddedType.toExternal U e)
+  def elimFun (α : U) : Bot U ⟶ α := HasEmbeddedBot.defElimFun α
+
+  def Not (α : U) : U := α ⟶ Bot U
 
 end HasEmbeddedBot
 
-class HasFunctorialBot (U : Universe.{u}) [HasEmbeddedFunctors.{u, w} U]
-  extends HasEmbeddedBot U where
-(defElimFun (α : U) : HasEmbeddedBot.Bot U ⟶[λ e => HasEmbeddedBot.elim e] α)
-
-namespace HasFunctorialBot
-
-  variable {U : Universe} [HasEmbeddedFunctors U] [HasFunctorialBot U]
-
-  def elimFun (α : U) : HasEmbeddedBot.Bot U ⟶ α := HasFunctorialBot.defElimFun α
-
-  def Not (α : U) : U := α ⟶ HasEmbeddedBot.Bot U
-
-end HasFunctorialBot
-
-class HasClassicalLogic (U : Universe.{u}) [HasEmbeddedFunctors U] [HasFunctorialBot U] where
-(byContradictionFun (α : U) : HasFunctorialBot.Not (HasFunctorialBot.Not α) ⟶ α)
+class HasClassicalLogic (U : Universe.{u}) [HasEmbeddedFunctors.{u, w} U] [HasEmbeddedBot.{u, w} U] where
+(byContradictionFun (α : U) : HasEmbeddedBot.Not (HasEmbeddedBot.Not α) ⟶ α)
